theories/ftlr/interp_weakening.v
@@ -9,6 +9,7 @@ Section fundamental.
     {Σ:gFunctors}
     {ceriseg:ceriseG Σ} {sealsg: sealStoreG Σ}
     {Cname : CmptNameG}
+    {switcherg :switcherG}
     {stsg : STSG Addr region_type Σ} {heapg : heapGS Σ}
     {nainv: logrel_na_invs Σ}
     `{MP: MachineParameters}.
@@ -35,22 +36,38 @@ Section fundamental.
     iDestruct "Hinterp" as (rx' pw' dl' dro') "[%HEeq #Hinterp]"; inv HEeq.
     iExists rx',pw',dl',dro'.
     iSplit ; first done.
-    iModIntro.
-    rewrite /enter_cond /interp_expr /=.
-    iIntros (regs W' Hrelated).
-    destruct g.
-    - iAssert (future_world Global W W')%I as "%Hrelated'".
-      { iPureIntro.
-        apply related_sts_pub_priv_trans_world with W', related_sts_priv_refl_world; auto.
-      }
-      iSpecialize ("Hinterp" $! regs W' Hrelated').
-      iDestruct "Hinterp" as "[Hinterp Hinterp_borrowed]".
-      iSplitL; iFrame "#".
-    - iAssert (future_world Local W W')%I as "%Hrelated'".
+
+    rewrite (decide_False (P := WCap _ Local _ _ _ = _)).
+    2:{ rewrite switcher_ret_correct; intros; congruence. }
+
+    destruct (decide (WCap (E rx' pw' dl' dro') g b e a = switcher_ret_entry_point)).
+    - iModIntro.
+      iDestruct "Hinterp" as "#Hinterp".
+      rewrite switcher_ret_correct in e0 ; simplify_eq.
+      rewrite /enter_cond /switcher_cond /interp_expr /=.
+      iIntros (regs W' Hrelated).
+      iAssert (future_world Local W W')%I as "%Hrelated'".
       { done. }
       iSpecialize ("Hinterp" $! regs W' Hrelated').
       iDestruct "Hinterp" as "[Hinterp Hinterp_borrowed]".
       iSplitL; iFrame "#".
+    - iModIntro.
+      iDestruct "Hinterp" as "#Hinterp".
+      rewrite /enter_cond /interp_expr /=.
+      iIntros (regs W' Hrelated).
+      destruct g.
+      + iAssert (future_world Global W W')%I as "%Hrelated'".
+        { iPureIntro.
+          apply related_sts_pub_priv_trans_world with W', related_sts_priv_refl_world; auto.
+        }
+        iSpecialize ("Hinterp" $! regs W' Hrelated').
+        iDestruct "Hinterp" as "[Hinterp Hinterp_borrowed]".
+        iSplitL; iFrame "#".
+      + iAssert (future_world Local W W')%I as "%Hrelated'".
+        { done. }
+        iSpecialize ("Hinterp" $! regs W' Hrelated').
+        iDestruct "Hinterp" as "[Hinterp Hinterp_borrowed]".
+        iSplitL; iFrame "#".
   Qed.
 
   Lemma interp_weakeningEO W C p p' g g' b b' e e' a a' :
@@ -81,7 +98,7 @@ Section fundamental.
     }
 
     case_eq (isWL p'); intros Hpwl'; auto.
-    - assert (isWL p = true) as Hpwl by (destruct_perm p; destruct_perm p'; naive_solver).
+    - assert (isWL p = true) as Hpwl by (clear -Hpwl' Hpwl_cond Hp ; destruct_perm p; destruct_perm p'; naive_solver).
       rewrite Hpwl in Hpwl_cond.
       destruct g; try congruence.
       destruct g'; simpl in Hl; try tauto.
@@ -138,6 +155,14 @@ Section fundamental.
   Proof.
     intros HpnotSentry HpnotO Hb He Hp Hl.
     iIntros "#IH HA".
+    destruct (decide ((WCap (E rx pw dl dro) g' b' e' a') = switcher_ret_entry_point) ).
+    { rewrite switcher_ret_correct in e0; simplify_eq.
+      destruct p; cbn in Hp; iExFalso; last by cbn in HpnotSentry.
+      rewrite Is_true_true in Hp.
+      do 4 (apply andb_true_iff in Hp; destruct Hp as [Hp _]).
+      destruct rx; try congruence.
+      by rewrite !fixpoint_interp1_eq /=.
+    }
     rewrite !fixpoint_interp1_eq !interp1_eq.
     rewrite HpnotO HpnotSentry.
     replace (isO (E rx pw dl dro)) with false ; auto.
@@ -146,6 +171,7 @@ Section fundamental.
     iDestruct "HA" as "[#A %Hpwl_cond]".
     iExists rx,pw,dl,dro.
     iSplit ; first done.
+    rewrite decide_False ; last done.
     iModIntro.
     rewrite /enter_cond /interp_expr /=.
     iIntros (r W') "#Hfuture".
@@ -334,10 +360,9 @@ Section fundamental.
     opose proof (HpersP (W,C,_)) as HpersPborrowed; cbn in HpersPborrowed.
     iDestruct "HPborrowed" as "#HPborrowed".
     replace (borrow (WSealable (borrow_sb sb)))
-      with (WSealable (borrow_sb sb)).
+      with (WSealable (borrow_sb sb))
+           by (cbn; destruct sb; auto).
     iFrame "∗#%".
-    cbn.
-    destruct sb; auto.
   Qed.
 
   (* TODO move in machine_base *)
@@ -493,24 +518,42 @@ Section fundamental.
       + iIntros (w W0 W1 Hrelated); iModIntro.
         iIntros "Hinterp".
         iApply interp_monotone; eauto.
-      + iIntros (w W0 W1 HcanStore Hrelated); iModIntro.
+      + iIntros (w).
+        destruct (decide (w = switcher_ret_entry_point)) as [-> | Hneq_switcher]; cycle 1.
+        * iIntros ([HcanStore _]).
+          rewrite /future_priv_mono.
+          rewrite decide_False //.
+          iIntros (W0 W1 _ Hrelated); iModIntro.
+          iIntros "Hinterp".
+          iApply interp_monotone_nl; eauto.
+          iPureIntro; cbn.
+          by eapply canStore_global_nonisWL.
+        * iIntros (W0 W1 Hrelated); iModIntro.
+          iIntros "Hinterp".
+          iApply interp_monotone; eauto.
+    - ospecialize (Hρ _); first done.
+      iIntros (w).
+      destruct (decide (w = switcher_ret_entry_point)) as [-> | Hneq_switcher]; cycle 1.
+      * iIntros ([HcanStore _]).
+        rewrite /future_priv_mono.
+        rewrite decide_False //.
+        iIntros (W0 W1 _ Hrelated); iModIntro.
         iIntros "Hinterp".
         iApply interp_monotone_nl; eauto.
         iPureIntro; cbn.
         by eapply canStore_global_nonisWL.
-    - ospecialize (Hρ _); first done.
-      iIntros (w W0 W1 HcanStore Hrelated); iModIntro.
-      iIntros "Hinterp".
-      iApply interp_monotone_nl; eauto.
-      iPureIntro; cbn.
-      by eapply canStore_global_nonisWL.
+      * iIntros (W0 W1 Hrelated); iModIntro.
+        iIntros "Hinterp".
+        iApply interp_monotone; eauto.
   Qed.
 
   Lemma future_priv_mono_interp_z (C : CmptName) (z : Z) :
     ⊢ future_priv_mono C interpC (WInt z).
   Proof.
+    rewrite /future_priv_mono switcher_ret_correct.
+    rewrite decide_False //.
     iModIntro.
-    iIntros (W W') "%Hrelated Hinterp".
+    iIntros (W W' _) "%Hrelated Hinterp".
     cbn; iEval (rewrite fixpoint_interp1_eq); done.
   Qed.
 
