theories/region_invariants_revocation.v
@@ -7,6 +7,7 @@ Section heap.
   Context {Σ:gFunctors}
     {ceriseg:ceriseG Σ}
     {Cname : CmptNameG}
+    {switcherg :switcherG}
     {stsg : STSG Addr region_type Σ}
     {heapg : heapGS Σ}
     `{MP: MachineParameters}.
@@ -145,6 +146,66 @@ Section heap.
     - repeat rewrite insert_insert dom_insert_L;rewrite Hdom';set_solver.
   Qed.
 
+  Lemma update_region_revoked_temp_switcher_updated E W C a p v φ `{∀ Wv, Persistent (φ Wv)} :
+    let W' := (<s[ a := Temporary ]s> W) in
+    (std W) !! a = Some Revoked →
+    isO p = false → v = switcher_ret_entry_point →
+
+    future_pub_mono C φ v -∗
+    sts_full_world W C -∗
+    region W C -∗
+    a ↦ₐ v -∗
+    φ (W',C, v) -∗
+    rel C a p φ
+
+    ={E}=∗
+
+    region W' C
+    ∗ sts_full_world W' C.
+  Proof.
+    intro.
+    iIntros (Hrev Hne His_switcher) "#HmonoV Hsts Hreg Hl #Hφ #Hrel".
+    rewrite region_eq /region_def.
+    iDestruct "Hreg" as (M Mρ) "(Hγrel & %Hdom & %Hdom' & Hpreds)";simplify_eq.
+    rewrite rel_eq /rel_def. iDestruct "Hrel" as (γ) "[HREL Hsaved]".
+    iDestruct ( (reg_in C M) with "[$HREL $Hγrel]") as %HMeq;eauto.
+    rewrite /region_map_def HMeq big_sepM_insert; [|by rewrite lookup_delete].
+    iDestruct "Hpreds" as "[Hl' Hr]".
+    iDestruct "Hl'" as (ρ Hl) "[Hstate Hresources]".
+    iDestruct (sts_full_state_std with "Hsts Hstate") as %Hρ.
+    rewrite Hrev in Hρ. inversion Hρ as [Hρrev]. subst.
+    iMod (sts_update_std _ _ _ _ Temporary with "Hsts Hstate") as "[Hsts Hstate]".
+    assert (related_sts_pub_world W (<s[a := Temporary ]s> W)) as Hrelated.
+    { apply related_sts_pub_revoked_temp; auto. }
+    iDestruct (region_map_monotone _ _ _ _ _ Hrelated with "Hr") as "Hr".
+    assert (is_Some (M !! a)) as [x Hsome].
+    { apply elem_of_dom. rewrite -Hdom. rewrite elem_of_dom. done. }
+    iDestruct (region_map_delete_nonfrozen with "Hr") as "Hr"; [intros m;congruence|].
+    iDestruct (region_map_insert_nonfrozen _ _ _ _ _ Temporary with "Hr") as "Hr";auto.
+    iDestruct (big_sepM_delete _ _ a _ Hsome with "[Hl Hstate $Hr]") as "Hr".
+    { iExists Temporary. iFrame. iSplitR;[iPureIntro;apply lookup_insert|].
+      iExists γ, p, φ. rewrite HMeq lookup_insert in Hsome.
+      inversion Hsome.
+      repeat (iSplit; auto).
+      destruct (isWL p); auto.
+      rewrite /future_priv_mono.
+      rewrite decide_True ; done.
+    }
+    subst W'.
+    iFrame "Hsts".
+    iExists M.
+    rewrite -HMeq.
+    iFrame "∗%".
+    iPureIntro.
+    rewrite /std.
+    apply insert_id in Hsome; rewrite -Hsome.
+    apply insert_id in Hl; rewrite -Hl.
+    split.
+    - repeat rewrite dom_insert_L;rewrite Hdom;set_solver.
+    - repeat rewrite insert_insert dom_insert_L;rewrite Hdom';set_solver.
+  Qed.
+
+
   Lemma update_region_revoked_temp_nwl_updated E W C a p v φ `{∀ Wv, Persistent (φ Wv)} :
     let W' := (<s[ a := Temporary ]s> W) in
     (std W) !! a = Some Revoked →
@@ -186,6 +247,66 @@ Section heap.
       iExists γ, p, φ. rewrite HMeq lookup_insert in Hsome.
       inversion Hsome. rewrite Hpwl.
       repeat (iSplit; auto).
+    }
+    subst W'.
+    iFrame "Hsts".
+    iExists M.
+    rewrite -HMeq.
+    iFrame "∗%".
+    iPureIntro.
+    rewrite /std.
+    apply insert_id in Hsome; rewrite -Hsome.
+    apply insert_id in Hl; rewrite -Hl.
+    split.
+    - repeat rewrite dom_insert_L;rewrite Hdom;set_solver.
+    - repeat rewrite insert_insert dom_insert_L;rewrite Hdom';set_solver.
+  Qed.
+
+  Lemma update_region_revoked_temp_pre_nwl_updated E W C a p v φ `{∀ Wv, Persistent (φ Wv)} :
+    let W' := (<s[ a := Temporary ]s> W) in
+    (std W) !! a = Some Revoked →
+    isO p = false → isWL p = false →
+    v ≠ switcher_ret_entry_point ->
+
+    future_priv_mono_pre C φ v -∗
+    sts_full_world W C -∗
+    region W C -∗
+    a ↦ₐ v -∗
+    φ (W',C, v) -∗
+    rel C a p φ
+
+    ={E}=∗
+
+    region W' C
+    ∗ sts_full_world W' C.
+  Proof.
+    intro.
+    iIntros (Hrev Hne Hpwl Hnswitcher) "#HmonoV Hsts Hreg Hl #Hφ #Hrel".
+    rewrite region_eq /region_def.
+    iDestruct "Hreg" as (M Mρ) "(Hγrel & %Hdom & %Hdom' & Hpreds)";simplify_eq.
+    rewrite rel_eq /rel_def. iDestruct "Hrel" as (γ) "[HREL Hsaved]".
+    iDestruct ( (reg_in C M) with "[$HREL $Hγrel]") as %HMeq;eauto.
+    rewrite /region_map_def HMeq big_sepM_insert; [|by rewrite lookup_delete].
+    iDestruct "Hpreds" as "[Hl' Hr]".
+    iDestruct "Hl'" as (ρ Hl) "[Hstate Hresources]".
+    iDestruct (sts_full_state_std with "Hsts Hstate") as %Hρ.
+    rewrite Hrev in Hρ. inversion Hρ as [Hρrev]. subst.
+    iMod (sts_update_std _ _ _ _ Temporary with "Hsts Hstate") as "[Hsts Hstate]".
+    assert (related_sts_pub_world W (<s[a := Temporary ]s> W)) as Hrelated.
+    { apply related_sts_pub_revoked_temp; auto. }
+    iDestruct (region_map_monotone _ _ _ _ _ Hrelated with "Hr") as "Hr".
+    assert (is_Some (M !! a)) as [x Hsome].
+    { apply elem_of_dom. rewrite -Hdom. rewrite elem_of_dom. done. }
+    iDestruct (region_map_delete_nonfrozen with "Hr") as "Hr"; [intros m;congruence|].
+    iDestruct (region_map_insert_nonfrozen _ _ _ _ _ Temporary with "Hr") as "Hr";auto.
+    iDestruct (big_sepM_delete _ _ a _ Hsome with "[Hl Hstate $Hr]") as "Hr".
+    { iExists Temporary. iFrame. iSplitR;[iPureIntro;apply lookup_insert|].
+      iExists γ, p, φ. rewrite HMeq lookup_insert in Hsome.
+      inversion Hsome. rewrite Hpwl.
+      repeat (iSplit; auto).
+      rewrite /future_priv_mono.
+      destruct ( decide (v = switcher_ret_entry_point) ) ; first congruence.
+      auto.
     }
     subst W'.
     iFrame "Hsts".
@@ -243,8 +364,14 @@ Section heap.
     iIntros (Hrev Hne Hpwl) "#HmonoV Hsts Hreg Hl #Hφ #Hrel".
     assert (related_sts_priv_world W (<s[ a := Temporary ]s> W)) as Hrelated.
     { apply related_sts_pub_priv_world,related_sts_pub_revoked_temp; auto. }
-    iDestruct ("HmonoV" $! W ((<s[ a := Temporary ]s> W)) with "[] [Hφ]") as "Hφ'"; eauto.
-    iApply (update_region_revoked_temp_nwl_updated with "HmonoV Hsts Hreg Hl Hφ' Hrel");auto.
+    assert (related_sts_pub_world W (<s[ a := Temporary ]s> W)) as Hrelated'.
+    { apply related_sts_pub_revoked_temp; auto. }
+    rewrite /future_priv_mono.
+    destruct (decide (v = switcher_ret_entry_point)); cycle 1.
+    - iDestruct ("HmonoV" $! W ((<s[ a := Temporary ]s> W)) with "[] [] [Hφ]") as "Hφ'"; eauto.
+      iApply (update_region_revoked_temp_pre_nwl_updated with "HmonoV Hsts Hreg Hl Hφ' Hrel");eauto.
+    - iDestruct ("HmonoV" $! W ((<s[ a := Temporary ]s> W)) with "[] [Hφ]") as "Hφ'"; eauto.
+      iApply (update_region_revoked_temp_switcher_updated with "HmonoV Hsts Hreg Hl Hφ' Hrel");eauto.
   Qed.
 
   (* -------------------------------------------------------------------------- *)
@@ -763,6 +890,7 @@ Section heap.
   (* ---------------------------------------------------------------------------------------- *)
   (* ------------------- IF THΕ FULL STS IS REVOKED, WΕ CAN REVOKE REGION ------------------- *)
 
+  (* TODO we maybe need a proof that the switcher_ret is valid in (revoke W) *)
   (* Note that Mρ by definition matches up with the full sts. Mρ starts out by being indirectly revoked *)
   Lemma monotone_revoke_region_def W C MC Mρ :
     ⌜dom (std W) = dom MC⌝
@@ -794,11 +922,15 @@ Section heap.
     iDestruct "Ha" as (γpred p φ) "(%Hγp & % & Hpred & Ha)".
     iDestruct "Ha" as (v Hne) "(Ha & #HmonoV & #Hφ)".
     iFrame "∗%#".
-    iNext. iApply ("HmonoV" with "[] Hφ").
-    iPureIntro.
-    apply revoke_related_sts_priv_world.
-    Unshelve. apply _.
-  Qed.
+    iNext.
+    rewrite /future_priv_mono.
+    destruct (decide (v = switcher_ret_entry_point)) as [-> |Hneqs_switcher]; cycle 1.
+    - iApply ("HmonoV" with "[] [] [$]"); eauto.
+      iPureIntro.
+      apply revoke_related_sts_priv_world.
+    - admit.
+      Unshelve. apply _.
+  Abort.
 
   (* ---------------------------------------------------------------------------------------- *)
   (* ------------------- A REVOKED W IS MONOTONE WRT PRIVATE FUTURE WORLD ------------------- *)
@@ -833,9 +965,11 @@ Section heap.
     iDestruct "Ha" as (γpred p φ) "(%Hγp & % & Hpred & Ha)".
     iDestruct "Ha" as (v Hne) "(Ha & #HmonoV & #Hφ)".
     iFrame "∗%#".
-    iNext. iApply "HmonoV";[|iFrame "#"]. auto.
+    iNext.
+    (* iApply "HmonoV";[|iFrame "#"]. auto. *)
+    admit.
     Unshelve. apply _.
-  Qed.
+  Abort.
 
   Lemma monotone_revoke_list_region_def_mono
     (W W1 W2: WORLD) (C : CmptName)
